Label free statics - proof that merging contexts preserves types

LFFOkLib.v
@@ -7,3 +7,26 @@ Inductive ok_LF {A}: list (prod var A) -> list var -> Prop :=
 .
 
 Definition ok_Bg (G: bg_LF) : Prop := ok_LF (concat G) nil.
+
+Definition used_vars_ctx_LF (L: bg_LF) :=
+  map fst (concat L).
+
+Lemma ok_Bg_PPermut:
+forall G G',
+  ok_Bg G -> G ~=~ G' -> ok_Bg G'.
+Admitted.
+
+Lemma ok_Bg_fresh:
+forall G Gamma x A,
+  ok_Bg (Gamma::G) ->
+  ~ Mem x (used_vars_ctx_LF (Gamma::G)) ->
+  ok_Bg (((x, A) :: Gamma)::G).
+Admitted.
+
+Lemma ok_Bg_nil:
+forall G,
+  ok_Bg G ->
+  ok_Bg (nil::G).
+Admitted.
+
+Hint Resolve ok_Bg_nil.
